---
title: "An experiemental post"
date: 2019-11-13T15:34:30+10:00
last_modified_at: 2021-09-30T12:00:00+10:00
categories:
  - blog
tags:
  - experiments
---

# Summary

This post is solely an experiment with a number of different markdown features to see how well they work. This page should not be taken seriously by the general reader but simply be understood as an experimental wasteland of information. Enjoy!

# Maths

The following equations demonstrate the process of completing the square of a quadratic equation to get to the solutions for x.

**Primary Notice:** Mathjax should now be working on this page. Fingers crossed ðŸ¤ž. (with scripts.html, not script.html **and** the math now working properly with brackets and script updated (twice).)
{: .notice--primary}

$$
\begin{aligned}
  x^2+6x-11=0 \\
  x^2+6x+(\frac{6}{2})^2-(\frac{6}{2})^2-11=0 \\
  x^2+6x+3^2-3^2-11=0 \\
  (x+3)^2-9-11=0 \\
  (x+3)^2-20=0 \\
  (x+3)^2-(\sqrt{20})^2=0 \\
  (x+3-\sqrt{20})(x+3+\sqrt{20})=0 \\
\end{aligned}
$$

From here, simply apply the **Null Factor Law** and you're all good!

$$
\begin{aligned}
  x+3-\sqrt{20} = 0 \\
  x = -3+\sqrt{20} \\
\end{aligned}
$$

Therefore, the two solutions to $$ x^2+6x-11=0 $$ are $$ x=-3+\sqrt{20} $$ and $$ x=-3-\sqrt{20} $$, or more concisely, $$ x=-3 \pm \sqrt{20} $$.